Rewrite.

theories/zoo_std/xchain.v
@@ -19,7 +19,7 @@ Implicit Types v next dst : val.
 Section zoo_G.
   Context `{zoo_G : !ZooG Σ}.
 
-  Fixpoint xchain_model nodes dst : iProp Σ :=
+  Fixpoint xchain nodes dst : iProp Σ :=
     match nodes with
     | [] =>
         True
@@ -29,71 +29,71 @@ Section zoo_G.
             node.[xchain_next] ↦ dst
         | node' :: _ =>
             node.[xchain_next] ↦ #node' ∗
-            xchain_model nodes dst
+            xchain nodes dst
         end
     end.
-  #[global] Arguments xchain_model !_ _ / : assert.
+  #[global] Arguments xchain !_ _ / : assert.
 
-  #[global] Instance xchain_model_timeless nodes dst :
-    Timeless (xchain_model nodes dst).
+  #[global] Instance xchain_timeless nodes dst :
+    Timeless (xchain nodes dst).
   Proof.
     induction nodes as [| ? []]; apply _.
   Qed.
 
-  Lemma xchain_model_nil dst :
-    ⊢ xchain_model [] dst.
+  Lemma xchain_nil dst :
+    ⊢ xchain [] dst.
   Proof.
     iSteps.
   Qed.
 
-  Lemma xchain_model_singleton node dst :
-    xchain_model [node] dst ⊣⊢
+  Lemma xchain_singleton node dst :
+    xchain [node] dst ⊣⊢
     node.[xchain_next] ↦ dst.
   Proof.
     iSteps.
   Qed.
-  Lemma xchain_model_singleton_1 node dst :
-    xchain_model [node] dst ⊢
+  Lemma xchain_singleton_1 node dst :
+    xchain [node] dst ⊢
     node.[xchain_next] ↦ dst.
   Proof.
     iSteps.
   Qed.
-  Lemma xchain_model_singleton_2 node dst :
+  Lemma xchain_singleton_2 node dst :
     node.[xchain_next] ↦ dst ⊢
-    xchain_model [node] dst.
+    xchain [node] dst.
   Proof.
     iSteps.
   Qed.
 
-  Lemma xchain_model_cons nodes node nodes' dst :
+  Lemma xchain_cons nodes node nodes' dst :
     nodes = node :: nodes' →
-    xchain_model nodes dst ⊣⊢
+    xchain nodes dst ⊣⊢
       node.[xchain_next] ↦ from_option #@{location} dst (head nodes') ∗
-      xchain_model nodes' dst.
+      xchain nodes' dst.
   Proof.
     destruct nodes'; iSteps.
   Qed.
-  Lemma xchain_model_cons_1 nodes node nodes' dst :
+  Lemma xchain_cons_1 nodes node nodes' dst :
     nodes = node :: nodes' →
-    xchain_model nodes dst ⊢
+    xchain nodes dst ⊢
       node.[xchain_next] ↦ from_option #@{location} dst (head nodes') ∗
-      xchain_model nodes' dst.
+      xchain nodes' dst.
   Proof.
-    intros. rewrite xchain_model_cons //.
+    intros. rewrite xchain_cons //.
   Qed.
-  Lemma xchain_model_cons_2 node nodes dst :
+  Lemma xchain_cons_2 node nodes dst :
     node.[xchain_next] ↦ from_option #@{location} dst (head nodes) -∗
-    xchain_model nodes dst -∗
-    xchain_model (node :: nodes) dst.
+    xchain nodes dst -∗
+    xchain (node :: nodes) dst.
   Proof.
-    rewrite (xchain_model_cons (node :: nodes)) //. iSteps.
+    rewrite (xchain_cons (node :: nodes)) //. iSteps.
   Qed.
 
-  Lemma xchain_model_app nodes nodes1 nodes2 dst :
+  Lemma xchain_app nodes nodes1 nodes2 dst :
     nodes = nodes1 ++ nodes2 →
-    xchain_model nodes dst ⊣⊢
-      xchain_model nodes1 (from_option #@{location} dst (head nodes2)) ∗
-      xchain_model nodes2 dst.
+    xchain nodes dst ⊣⊢
+      xchain nodes1 (from_option #@{location} dst (head nodes2)) ∗
+      xchain nodes2 dst.
   Proof.
     intros ->.
     iInduction nodes1 as [| node1 [| node1' nodes1]] "IH".
@@ -105,92 +105,92 @@ Section zoo_G.
       + iIntros "(($ & H1) & H2)".
         iApply ("IH" with "[$H1 $H2]").
   Qed.
-  Lemma xchain_model_app_1 nodes nodes1 nodes2 dst :
+  Lemma xchain_app_1 nodes nodes1 nodes2 dst :
     nodes = nodes1 ++ nodes2 →
-    xchain_model nodes dst ⊢
-      xchain_model nodes1 (from_option #@{location} dst (head nodes2)) ∗
-      xchain_model nodes2 dst.
+    xchain nodes dst ⊢
+      xchain nodes1 (from_option #@{location} dst (head nodes2)) ∗
+      xchain nodes2 dst.
   Proof.
-    intros. rewrite xchain_model_app //.
+    intros. rewrite xchain_app //.
   Qed.
-  Lemma xchain_model_app_2 nodes1 nodes2 dst :
-    xchain_model nodes1 (from_option #@{location} dst (head nodes2)) -∗
-    xchain_model nodes2 dst -∗
-    xchain_model (nodes1 ++ nodes2) dst.
+  Lemma xchain_app_2 nodes1 nodes2 dst :
+    xchain nodes1 (from_option #@{location} dst (head nodes2)) -∗
+    xchain nodes2 dst -∗
+    xchain (nodes1 ++ nodes2) dst.
   Proof.
-    rewrite (xchain_model_app (nodes1 ++ nodes2)) //. iSteps.
+    rewrite (xchain_app (nodes1 ++ nodes2)) //. iSteps.
   Qed.
 
-  Lemma xchain_model_snoc nodes nodes' node dst :
+  Lemma xchain_snoc nodes nodes' node dst :
     nodes = nodes' ++ [node] →
-    xchain_model nodes dst ⊣⊢
-      xchain_model nodes' #node ∗
+    xchain nodes dst ⊣⊢
+      xchain nodes' #node ∗
       node.[xchain_next] ↦ dst.
   Proof.
-    intros. rewrite xchain_model_app //.
+    intros. rewrite xchain_app //.
   Qed.
-  Lemma xchain_model_snoc_1 nodes nodes' node dst :
+  Lemma xchain_snoc_1 nodes nodes' node dst :
     nodes = nodes' ++ [node] →
-    xchain_model nodes dst ⊢
-      xchain_model nodes' #node ∗
+    xchain nodes dst ⊢
+      xchain nodes' #node ∗
       node.[xchain_next] ↦ dst.
   Proof.
-    intros. rewrite xchain_model_snoc //.
+    intros. rewrite xchain_snoc //.
   Qed.
-  Lemma xchain_model_snoc_2 nodes node dst :
-    xchain_model nodes #node -∗
+  Lemma xchain_snoc_2 nodes node dst :
+    xchain nodes #node -∗
     node.[xchain_next] ↦ dst -∗
-    xchain_model (nodes ++ [node]) dst.
+    xchain (nodes ++ [node]) dst.
   Proof.
-    rewrite (xchain_model_snoc (nodes ++ [node])) //. iSteps.
+    rewrite (xchain_snoc (nodes ++ [node])) //. iSteps.
   Qed.
 
-  Lemma xchain_model_lookup {nodes} i node dst :
+  Lemma xchain_lookup {nodes} i node dst :
     nodes !! i = Some node →
-    xchain_model nodes dst ⊣⊢
-      xchain_model (take i nodes) #node ∗
+    xchain nodes dst ⊣⊢
+      xchain (take i nodes) #node ∗
       node.[xchain_next] ↦ from_option #@{location} dst (nodes !! S i) ∗
-      xchain_model (drop (S i) nodes) dst.
+      xchain (drop (S i) nodes) dst.
   Proof.
     intros Hlookup.
     pose proof Hlookup as Hnodes%take_drop_middle.
-    rewrite -{1}Hnodes xchain_model_app // (xchain_model_cons (node :: _)) // head_drop //.
+    rewrite -{1}Hnodes xchain_app // (xchain_cons (node :: _)) // head_drop //.
   Qed.
-  Lemma xchain_model_lookup_1 {nodes} i node dst :
+  Lemma xchain_lookup_1 {nodes} i node dst :
     nodes !! i = Some node →
-    xchain_model nodes dst ⊢
-      xchain_model (take i nodes) #node ∗
+    xchain nodes dst ⊢
+      xchain (take i nodes) #node ∗
       node.[xchain_next] ↦ from_option #@{location} dst (nodes !! S i) ∗
-      xchain_model (drop (S i) nodes) dst.
+      xchain (drop (S i) nodes) dst.
   Proof.
-    intros. rewrite xchain_model_lookup //.
+    intros. rewrite xchain_lookup //.
   Qed.
-  Lemma xchain_model_lookup_2 {nodes} i node next dst :
+  Lemma xchain_lookup_2 {nodes} i node next dst :
     nodes !! i = Some node →
     next = from_option #@{location} dst (nodes !! S i) →
-    xchain_model (take i nodes) #node -∗
+    xchain (take i nodes) #node -∗
     node.[xchain_next] ↦ next -∗
-    xchain_model (drop (S i) nodes) dst -∗
-    xchain_model nodes dst.
+    xchain (drop (S i) nodes) dst -∗
+    xchain nodes dst.
   Proof.
-    intros. rewrite (@xchain_model_lookup nodes) //. iSteps.
+    intros. rewrite (@xchain_lookup nodes) //. iSteps.
   Qed.
 
-  Lemma xchain_model_lookup_acc {nodes} i node dst :
+  Lemma xchain_lookup_acc {nodes} i node dst :
     nodes !! i = Some node →
-    xchain_model nodes dst ⊢
+    xchain nodes dst ⊢
       node.[xchain_next] ↦ from_option #@{location} dst (nodes !! S i) ∗
       ( node.[xchain_next] ↦ from_option #@{location} dst (nodes !! S i) -∗
-        xchain_model nodes dst
+        xchain nodes dst
       ).
   Proof.
-    intros. rewrite xchain_model_lookup //. iSteps.
+    intros. rewrite xchain_lookup //. iSteps.
   Qed.
 
-  Lemma xchain_model_exclusive nodes dst1 dst2 :
+  Lemma xchain_exclusive nodes dst1 dst2 :
     0 < length nodes →
-    xchain_model nodes dst1 -∗
-    xchain_model nodes dst2 -∗
+    xchain nodes dst1 -∗
+    xchain nodes dst2 -∗
     False.
   Proof.
     iIntros "% H1 H2".
@@ -200,8 +200,8 @@ Section zoo_G.
     all: iApply (pointsto_exclusive with "H1 H2").
   Qed.
 
-  Lemma xchain_model_NoDup nodes dst :
-    xchain_model nodes dst ⊢
+  Lemma xchain_NoDup nodes dst :
+    xchain nodes dst ⊢
     ⌜NoDup nodes⌝.
   Proof.
     rewrite NoDup_alt.
@@ -211,8 +211,8 @@ Section zoo_G.
     { destruct (Nat.min_spec i1 i2) as [(_ & ->) | (_ & ->)]; done. }
     assert (nodes !! (i1 `max` i2) = Some node) as Hlookup_max.
     { destruct (Nat.max_spec i1 i2) as [(_ & ->) | (_ & ->)]; done. }
-    iDestruct (xchain_model_lookup (i1 `min` i2) with "H") as "(_ & Hnode_1 & H)"; first done.
-    iDestruct (xchain_model_lookup (i1 `max` i2 - i1 `min` i2 - 1) node with "H") as "(_ & Hnode_2 & _)".
+    iDestruct (xchain_lookup (i1 `min` i2) with "H") as "(_ & Hnode_1 & H)"; first done.
+    iDestruct (xchain_lookup (i1 `max` i2 - i1 `min` i2 - 1) node with "H") as "(_ & Hnode_2 & _)".
     { rewrite lookup_drop -Hlookup_max. f_equal. lia. }
     iApply (pointsto_exclusive with "Hnode_1 Hnode_2").
   Qed.
@@ -220,12 +220,12 @@ Section zoo_G.
   Lemma xchain_next_spec {nodes node} nodes' dst E :
     nodes = node :: nodes' →
     {{{
-      xchain_model nodes dst
+      xchain nodes dst
     }}}
       (#node).{xchain_next} @ E
     {{{
       RET from_option #@{location} dst (head nodes');
-      xchain_model nodes dst
+      xchain nodes dst
     }}}.
   Proof.
     iIntros (->) "%Φ H HΦ".
@@ -234,29 +234,29 @@ Section zoo_G.
   Lemma xchain_next_spec_lookup {nodes} i node dst E :
     nodes !! i = Some node →
     {{{
-      xchain_model nodes dst
+      xchain nodes dst
     }}}
       (#node).{xchain_next} @ E
     {{{
       RET from_option #@{location} dst (nodes !! S i);
-      xchain_model nodes dst
+      xchain nodes dst
     }}}.
   Proof.
     intros Hlookup.
-    setoid_rewrite xchain_model_lookup_acc at 1; last done.
+    setoid_rewrite xchain_lookup_acc at 1; last done.
     iSteps.
   Qed.
 
   Lemma xchain_set_next_spec {nodes node} nodes' dst v E :
     nodes = node :: nodes' →
     {{{
-      xchain_model nodes dst
+      xchain nodes dst
     }}}
       (#node) <-{xchain_next} v @ E
     {{{
       RET ();
-      xchain_model [node] v ∗
-      xchain_model nodes' dst
+      xchain [node] v ∗
+      xchain nodes' dst
     }}}.
   Proof.
     iIntros (->) "%Φ H HΦ".
@@ -265,22 +265,22 @@ Section zoo_G.
   Lemma xchain_set_next_spec_lookup {nodes} i node dst v E :
     nodes !! i = Some node →
     {{{
-      xchain_model nodes dst
+      xchain nodes dst
     }}}
       #node <-{xchain_next} v @ E
     {{{
       RET ();
-      xchain_model (take (S i) nodes) v ∗
-      xchain_model (drop (S i) nodes) dst
+      xchain (take (S i) nodes) v ∗
+      xchain (drop (S i) nodes) dst
     }}}.
   Proof.
     intros Hlookup.
-    setoid_rewrite xchain_model_lookup at 1; last done.
+    setoid_rewrite xchain_lookup at 1; last done.
     iIntros "%Φ (H1 & Hnode & H2) HΦ".
     wp_store.
-    iDestruct (xchain_model_snoc_2 with "H1 Hnode") as "H1".
+    iDestruct (xchain_snoc_2 with "H1 Hnode") as "H1".
     rewrite -take_S_r //. iSteps.
   Qed.
 End zoo_G.
 
-#[global] Opaque xchain_model.
+#[global] Opaque xchain.
